src/goose_lang/lib/atomic/atomic.v
@@ -1,0 +1,96 @@
+From stdpp Require Import namespaces.
+From iris.proofmode Require Import tactics.
+From iris.algebra Require Import excl.
+From Perennial.base_logic.lib Require Import invariants.
+From Perennial.program_logic Require Import weakestpre.
+
+From Perennial.goose_lang Require Import lang typing.
+From Perennial.goose_lang Require Import proofmode notation.
+From Perennial.goose_lang.lib Require Import typed_mem.
+From Perennial.goose_lang.lib Require Export atomic.impl.
+Set Default Proof Using "Type".
+
+Section goose_lang.
+Context `{ffi_sem: ffi_semantics}.
+Context `{!ffi_interp ffi}.
+Context {ext_tys: ext_types ext}.
+
+Section proof.
+Context `{!heapGS Σ} (N : namespace).
+
+#[local] Lemma uint64_pointsto (l: loc) (x: w64) :
+  l ↦[uint64T] #x ⊣⊢ heap_pointsto l (DfracOwn 1) #x.
+Proof.
+  rewrite struct_pointsto_eq /struct_pointsto_def /=.
+  rewrite loc_add_0 right_id.
+  iSplit.
+  - iIntros "[$ _]".
+  - iIntros "$".
+    iPureIntro. val_ty.
+Qed.
+
+#[local] Lemma uint32_pointsto (l: loc) (x: w32) :
+  l ↦[uint32T] #x ⊣⊢ heap_pointsto l (DfracOwn 1) #x.
+Proof.
+  rewrite struct_pointsto_eq /struct_pointsto_def /=.
+  rewrite loc_add_0 right_id.
+  iSplit.
+  - iIntros "[$ _]".
+  - iIntros "$".
+    iPureIntro. val_ty.
+Qed.
+
+Lemma wp_LoadUint64 (l: loc) (x: w64) stk E :
+  {{{ ▷l ↦[uint64T] #x }}}
+    atomic.LoadUint64 #l @ stk; E
+  {{{ RET #x; l ↦[uint64T] #x }}}.
+Proof.
+  rewrite /atomic.LoadUint64.
+  setoid_rewrite uint64_pointsto.
+  iIntros (Φ) "Hl HΦ".
+  wp_pures.
+  wp_apply (wp_load with "[$Hl]"). iIntros "Hl".
+  iApply "HΦ". iFrame.
+Qed.
+
+Lemma wp_LoadUint32 (l: loc) (x: w32) stk E :
+  {{{ ▷l ↦[uint32T] #x }}}
+    atomic.LoadUint32 #l @ stk; E
+  {{{ RET #x; l ↦[uint32T] #x }}}.
+Proof.
+  rewrite /atomic.LoadUint32 /atomic.LoadUint64.
+  setoid_rewrite uint32_pointsto.
+  iIntros (Φ) "Hl HΦ".
+  wp_pures.
+  wp_apply (wp_load with "[$Hl]"). iIntros "Hl".
+  iApply "HΦ". iFrame.
+Qed.
+
+Lemma wp_StoreUint64 (l: loc) (x0 x: w64) stk E :
+  {{{ ▷l ↦[uint64T] #x0 }}}
+    atomic.StoreUint64 #l #x @ stk; E
+  {{{ RET #(); l ↦[uint64T] #x }}}.
+Proof.
+  rewrite /atomic.StoreUint64.
+  setoid_rewrite uint64_pointsto.
+  iIntros (Φ) "Hl HΦ".
+  wp_pures.
+  wp_apply (wp_atomic_store with "[$Hl]"). iIntros "Hl".
+  iApply "HΦ". iFrame.
+Qed.
+
+Lemma wp_StoreUint32 (l: loc) (x0 x: w32) stk E :
+  {{{ ▷l ↦[uint32T] #x0 }}}
+    atomic.StoreUint32 #l #x @ stk; E
+  {{{ RET #(); l ↦[uint32T] #x }}}.
+Proof.
+  rewrite /atomic.StoreUint32 /atomic.StoreUint64.
+  setoid_rewrite uint32_pointsto.
+  iIntros (Φ) "Hl HΦ".
+  wp_pures.
+  wp_apply (wp_atomic_store with "[$Hl]"). iIntros "Hl".
+  iApply "HΦ". iFrame.
+Qed.
+
+End proof.
+End goose_lang.
