src/goose_lang/lib/atomic/impl.v
@@ -1,0 +1,24 @@
+From Perennial.goose_lang Require Import notation.
+
+(* this code is intended to be used qualified with the atomic module *)
+Module atomic.
+Section goose_lang.
+Context {ext:ffi_syntax}.
+
+Definition LoadUint64 : val :=
+  λ: "l", Load "l".
+
+Definition LoadUint32 : val := LoadUint64.
+
+Definition StoreUint64 : val :=
+  λ: "l" "x", AtomicStore "l" "x".
+
+Definition StoreUint32 : val := StoreUint64.
+
+Definition CompareAndSwapUint64 : val :=
+  λ: "l" "old" "new", CmpXchg "l" "old" "new".
+
+Definition CompareAndSwapUint32 : val := CompareAndSwapUint64.
+
+End goose_lang.
+End atomic.
